Extracted out more of GhostPtrToken proofs to use properties about GhostSeq and PermData

theories/typing/ghost.v
@@ -1,4 +1,4 @@
-From lrust.typing Require Export type.
+From lrust.typing Require Export type zst.
 From lrust.typing Require Import programs shr_bor own type_context product.
 Set Default Proof Using "Type".
 
@@ -7,18 +7,6 @@ Implicit Type 𝔄l: (list syn_type).
 
 Lemma proph_dep_ghost' {A} (vπ: proph A) ξl' ξl level: vπ ./{level} ξl → vπ ./{S level} ξl'.
 Proof. move=> H ?? Eqv. apply H. intros ?[? _]. apply Eqv. split. lia. right. lia. Qed.
-
-Fixpoint hrenew {A B: Type} (F: B → Type) (G: A → B) {Xl} (xl: hlist (F∘G) Xl)
-: hlist F (G<$>Xl).
-  destruct Xl. simpl. exact +[].
-  simpl. inversion xl. constructor. exact X0. apply hrenew. exact X1.
-Defined.
-
-Fixpoint hrenew' {A B: Type} (F: B → Type) (G: A → B) {Xl} (xl: hlist F (G<$>Xl))
-: hlist (F∘G) Xl.
-  destruct Xl. simpl. exact +[].
-  simpl. inversion xl. constructor. exact X0. apply hrenew'. exact X1.
-Defined.
 
 Definition prenew {A B: Type} (F: B → Type) (G: A → B) {Xl} (xl: plist (F∘G) Xl)
 : plist F (G<$>Xl).
@@ -73,8 +61,16 @@ End ghost.
 Section typing.
   Context `{!typeG Σ}.
 
+  Global Instance ghost_copy {𝔄} (ty: type 𝔄) : Copy (ghost ty) := _.
+
+  Global Instance ghost_sync {𝔄} (ty: type 𝔄) : Sync (ghost ty).
+  Proof. unfold ghost. done. Qed.
+
   Global Instance ghost_send {𝔄} (ty: type 𝔄) : Send (ghost ty).
   Proof. move=> Eq >/=. done. Qed.
+
+  Global Instance ghost_zst {𝔄} (ty: type 𝔄) : ZST (ghost ty).
+  Proof. done. Qed.
 
   Lemma ghost_resolve {𝔄} (ty: type 𝔄) E L : resolve E L (ghost ty) (const True).
   Proof. apply resolve_just. Qed.
@@ -104,28 +100,38 @@ Section typing.
     eqtype E L (&shr{κ} ty) (&shr{κ'} ty') f g.
   Proof. move=> [??] [??]. split; by apply shr_subtype. Qed. *)
 
-  Definition null_loc : loc := inhabitant.
-  Definition null_val : val := #null_loc.
-
-  Lemma ghost_new {𝔄} (ty: type 𝔄) κ E L p:
-    lctx_lft_alive E L (ty_lft (&shr{κ} ty)%T) →
-     typed_instr E L +[p ◁ (&shr{κ} ty)] Skip (λ _, +[null_val ◁ (box (ghost ty))]) id.
+  Lemma ghost_new_instr {𝔄} (ty: type 𝔄) p E L:
+    lctx_lft_alive E L (ty_lft ty%T) →
+     typed_instr E L +[p ◁ ty] (Skip ;; Skip) (const +[null_val ◁ (box (ghost ty)); p ◁ ty]) (λ post '-[x], post -[x; x]).
   Proof.
     intros Alv.
-    iIntros (??[aπ[]]) "LFT TIME _ _ E $ L [p _] Obs".
+    iIntros (??[aπ[]]) "LFT #TIME _ _ E $ L [p _] Obs".
     iMod (Alv with "E L") as (?) "[κ ToL]"; [done|].
-    iDestruct "p" as ([[]|][|]Ev) "[#⧖ ty]"=>//.
+    iDestruct "p" as (?? Ev) "[#⧖ ty]"=>//.
     iMod (ty_own_proph with "LFT [] ty κ") as "Upd";
       [done| iApply lft_incl_refl| ].
+    wp_bind Skip.
+    iApply (wp_persistent_time_receipt with "TIME ⧖"); [done|]. wp_seq. iIntros "⧖'". wp_seq.
     iApply (wp_step_fupdN_persistent_time_receipt _ _ ∅ with "TIME ⧖ [Upd]")=>//.
     { iApply step_fupdN_with_emp. by rewrite difference_empty_L.  }
-    wp_seq. iIntros "(%&%&%&ξl&tolft)".
-    iMod ("tolft" with "ξl") as "(_&lft)".
+    wp_seq. iIntros "(%&%&%&ξl&tolft)". 
+    iMod ("tolft" with "ξl") as "(ty&lft)".
     iMod ("ToL" with "lft") as "$".
-    iExists -[aπ]. iModIntro. iSplit. iSplit; [|done]. 
-    iExists _, _. iFrame "⧖". iSplit; [done|].
+    iExists -[aπ; aπ]. iModIntro. iSplit. iSplitR "ty". 
+    iExists _, _. iFrame "⧖'". iSplit; [done|].
     simpl. iSplit; [|done]. iNext. iExists _. iSplit; [by iApply heap_mapsto_vec_nil|].
-    iPureIntro. split; [done|]. eexists _. done. done.
+    iPureIntro. split; [done|]. eexists _. done.
+    iSplit; [|done]. rewrite tctx_hasty_val'; [|done]. iExists _. iFrame "⧖ ty".
+    done.
+  Qed.
+
+  Lemma ghost_new {𝔄 𝔅 𝔄l} (ty: type 𝔄) p E L (C: cctx 𝔅) (T: tctx 𝔄l) e tr:
+    Closed [] e → lctx_lft_alive E L (ty_lft ty%T) 
+     → typed_body E L C (null_val ◁ (box (ghost ty)) +:: p ◁ ty +:: T) e tr
+      -∗ typed_body E L C (p ◁ ty +:: T) ((Skip;;Skip) ;; e) (λ post '(x -:: rest), tr post (x -:: x -:: rest)).
+  Proof.
+    iIntros (??) "B". iApply type_seq; [by apply (ghost_new_instr ty)|apply tctx_incl_refl| |done].
+    intros ?[? ?]. done.
   Qed.
 
   Definition logic_fn {𝔄l 𝔅} (tyl: typel 𝔄l) (tyr: type 𝔅) (f: (plist of_syn_type 𝔄l) → 𝔅) :=
@@ -133,34 +139,42 @@ Section typing.
     (forallHL_1 (λ _ ty aπ, ∃ ξl, (ty_proph ty aπ ξl)) tyl aπl) 
     → ∃ ξl, (ty_proph tyr (λ π, f (papply aπl π)) ξl).
 
-  Definition tctx_ghost {𝔄l} (tyl: typel 𝔄l) := ((λ _ ty, null_val ◁ (box (ghost ty))) +<$> tyl).
+  Fixpoint tctx_ghost {𝔄l} (tyl: typel 𝔄l) (pl: plist (const path) 𝔄l)
+  : tctx ((ghostₛ 1)<$>𝔄l) :=
+    match tyl, pl with 
+      | +[], _ => +[]
+      | ty +:: tyl', p -::ps' => (p ◁ (box (ghost ty))) +:: tctx_ghost tyl' ps'
+    end.
 
-  Definition tctx_ghost' {𝔄l} (tyl: typel 𝔄l) :=
-    hrenew tctx_elt (ghostₛ 1) (tctx_ghost tyl).
-
-  Lemma logic_fn_ghost_tctx_incl {𝔄l 𝔅} (tyl: typel 𝔄l) (tyr: type 𝔅) f E L:
-   logic_fn tyl tyr f → tctx_incl E L (null_val ◁ (box ()) +:: (tctx_ghost' tyl)) +[null_val ◁ (box (ghost tyr))] (λ post '(_ -:: l), post (-[f (prenew' _ _ l)])).
+  Lemma logic_fn_ghost_tctx_incl {𝔄l 𝔅} (pl: plist (const path) 𝔄l) (tyl: typel 𝔄l) (tyr: type 𝔅) f E L:
+   logic_fn tyl tyr f → tctx_incl E L (null_val ◁ (box ()) +:: (tctx_ghost tyl pl)) +[null_val ◁ (box (ghost tyr))] (λ post '(_ -:: l), post (-[f (prenew' _ _ l)])).
   Proof. 
     unfold logic_fn. intros.
     (split; [solve_proper|]); iIntros (??[? vπl]?) "_ _ _ _ $ ty Obs"; iModIntro;  simpl.
     set pπ := ((prenew' _ _ vπl): plist (λ 𝔄, proph 𝔄) 𝔄l).
     iExists -[_]. iFrame "Obs". iSplit; [|done].
-    rewrite 2! (tctx_hasty_val null_val).
-    iDestruct "ty" as "((%&⧖&?)&ty)". destruct d; [done|].
+    rewrite 2! tctx_elt_interp_zst. 
+    iDestruct "ty" as "((%&⧖&_)&ty)".
     iExists _. iFrame "⧖". 
-    simpl. iSplit; [|done].
-    iAssert (▷⌜_⌝)%I with "[ty]" as ">X"; last first.
-    iAssert ⌜_⌝%I as %X. done. destruct (H pπ X).
-    iNext. iExists []. iSplit. by iApply heap_mapsto_vec_nil.
-    iPureIntro. split; [done|]. exists x. unfold pπ in H0.
-    revert H0. eassert (impl _ _); [|done]. f_equiv. 
-    fun_ext. intros. by rewrite prenew_apply'. clear H postπ f.
+    simpl. iSplit; [done|].
+    iAssert (▷⌜_⌝)%I with "[ty]" as "X"; last first. iStopProof.
+    f_equiv. f_equiv. intros ?. f_exact (H pπ H0). 
+    f_equiv. f_equiv. fun_ext=>?. by rewrite /pπ prenew_apply'.
+    clear H postπ f.
     iInduction tyl as [|? ?] "IH"; destruct vπl. iPureIntro. constructor.
-    rewrite /tctx_ghost' /tctx_ghost. simpl. rewrite (tctx_hasty_val null_val).
-    iDestruct "ty" as "((%&_&own)&ty)". destruct d0; [done|simpl].
-    iDestruct "own" as "((%&_&_&>%fst)&_)".
+    destruct pl; simpl. rewrite tctx_elt_interp_zst''.
+    iDestruct "ty" as "((%&%&_&_&_&>%fst)&ty)".
     iDestruct ("IH" with "ty") as ">%rest".
-    iNext. iPureIntro. unfold pπ. simpl. by constructor.
+    iNext. iPureIntro. done.
+  Qed.
+
+  Lemma logic_fn_ghost_tctx_incl' {𝔄 𝔄l 𝔅} (pl: plist (const path) (𝔄::𝔄l)) (ty: type 𝔄) (tyl: typel 𝔄l) (tyr: type 𝔅) f E L:
+   logic_fn (ty +:: tyl) tyr f → tctx_incl E L (tctx_ghost (ty +:: tyl) pl) +[null_val ◁ (box (ghost tyr))] (λ post l, post (-[f (prenew' _ _ l)])).
+  Proof. intros ?.
+    destruct pl; simpl.
+    eapply tctx_incl_ext. eapply tctx_incl_trans; [|eapply (logic_fn_ghost_tctx_incl ((phd -:: ptl): plist _ (𝔄::𝔄l))); done].
+    apply (tctx_incl_frame_r +[_] +[_; _] _). apply ghost_dummy'.
+    move=>?[??]/=. done.
   Qed.
 
 End typing.
