theories/typing/lib/ghostptrtoken/ghostptrtoken_merge.v
@@ -1,71 +1,29 @@
 From lrust.typing Require Export type.
-From lrust.typing Require Import uniq_util typing ptr.
-From lrust.typing.lib Require Import ghostptrtoken.ghostptrtoken ghostptrtoken.heap_util.
+From lrust.typing Require Import uniq_util typing ptr zst.
+From lrust.typing.lib.ghostptrtoken Require Import ghostptrtoken_basic heap_util ghostseq_basic.
 Set Default Proof Using "Type".
 
 Open Scope nat.
 Implicit Type 𝔄 𝔅: syn_type.
 
-Section ghostptrtoken_insertremove.
+Section ghostptrtoken_merge.
   Context `{!typeG Σ}.
 
   Definition ghostptrtoken_merge {𝔄} (ty: type 𝔄) : val :=
     fn: ["t"; "t2"] :=
+      Skip;;
       delete [ #1; "t"];;
-      return: ["t2"].
+      return: [null_val].
 
-  (* Rust's GhostPtrToken::merge *)
   Lemma ghostptrtoken_merge_type {𝔄} (ty: type 𝔄) :
-    typed_val (ghostptrtoken_merge ty) (fn<α>(∅; &uniq{α} (ghostptrtoken_ty ty), ghostptrtoken_ty ty) → ())
-      (λ post '-[(al, al'); al2], al' =  al2 ++ al → ((ty_size ty > 0) → NoDup al'.*1) → post ()).
+    (ty_size ty > 0)%Z → typed_val (ghostptrtoken_merge ty) (fn<α>(∅; &uniq{α} (ghostptrtoken_ty ty), ghostptrtoken_ty ty) → ())
+      (λ post '-[(al, al'); al2], al' = al2 ++ al → NoDup al'.*1 → post ()).
   Proof.
-    eapply type_fn; [apply _|]=> α ??[l[l2[]]]. simpl_subst.
-    iIntros (?(lπ & l2π &[]) ?) "#LFT #TIME #PROPH #UNIQ #E Na L C /=(l & l2 &_) #Obs".
-    rewrite !tctx_hasty_val. iDestruct "l" as ([|dl]) "[⧖1 l]"=>//.
-    case l as [[|l|]|]=>//. iDestruct "l" as "[(%ll & >↦l & [#LftIn uniq]) †l]".
-    case ll as [|[[|l'|]|][]]; try by iDestruct "uniq" as ">[]".
-    iDestruct "l2" as ([|dl2]) "[⧖2 l2]"=>//. case l2 as [[|l2|]|]=>//=.
-    iDestruct "l2" as "[l2' †l2]".
-    wp_bind (delete _). rewrite freeable_sz_full.
-    iApply ((wp_delete [ #l']) with "[↦l †l]"); [done| by iFrame|]. 
-    iNext. iIntros.
-    iDestruct "l2'" as (vl2) "(↦l2&l2')".
-    case dl2 as [|dl2]=>//=. iDestruct "l2'" as "(%aπl2&(->&->)&(↦2&†2))". 
-    iDestruct "uniq" as (du ξi [? Eq2]) "[Vo Bor]".
-    move: Eq2. set ξ := PrVar _ ξi=> Eq2.
-    iMod (lctx_lft_alive_tok α with "E L") as (?) "(α & L & ToL)"; [solve_typing..|].
-    iMod (bor_acc with "LFT Bor α") as "[(%&%& ⧖u & Pc & ↦token) ToBor]"; [done|].
-    wp_seq. iDestruct (uniq_agree with "Vo Pc") as %[<-<-].
-    rewrite split_mt_token. case du as [|du]=>//=.
-    iDestruct "↦token" as (aπl Eq1) "(↦l & ↦tys & †)".
-    iDestruct (persistent_time_receipt_mono (S (S du)) with "⧖1") as "⧖1". lia.
-    iCombine "⧖1 ⧖2" as "#⧖". simpl.
-    iMod (uniq_update with "UNIQ Vo Pc") as "[Vo Pc]"; [done|].
-    iAssert ((l' ↦∗: (ghostptrtoken_ty ty).(ty_own) _ (S (du `max` dl2)) tid))%I with "[↦l ↦tys † ↦2 †2]" as "own".
-    iExists _. iFrame. iExists (aπl2++aπl).
-    unfold big_sepAL. rewrite 2! big_sepL_app. iFrame. iSplit; [done|].
-    iNext. iSplitL "↦2";
-    iApply (big_sepL_impl with "[$]"); iModIntro; iIntros (?[??]?) "H";
-    iApply (ty_own_mt_depth_mono with "H"); lia.
-    iDestruct ((plain_entails_r (ghost_ptr_token_no_dup _ _ _ _ _)) with "own") as "(own&>%no_dup)".
-    iMod ("ToBor" with "[own Pc]") as "[Bor α]".
-    iDestruct (bi.later_intro with "own") as "own". 
-    iNext. iExists _, _. iFrame "⧖ Pc own".
-    iMod ("ToL" with "α L") as "L".
-    set lπ' := λ π, ((alapply (aπl2++aπl) π), π ξ).
-    iApply (type_type +[#l' ◁ &uniq{α} (ghostptrtoken_ty ty); #l2 ◁ box ()] -[lπ'; const ()]
-    with "[] LFT TIME PROPH UNIQ E Na L C [-] []").
-    - iApply type_jump; [solve_typing|solve_extract|solve_typing].
-    - iSplitL "Vo Bor"; [|iSplitL; [|done]]. rewrite (tctx_hasty_val #l').
-      iExists _. iSplit; [done|]. 
-      iSplit; [done|]. fold max. iExists _, _. rewrite /uniq_body.
-      rewrite (proof_irrel (@prval_to_inh (listₛ (locₛ * 𝔄)) (fst ∘ lπ')) (@prval_to_inh (listₛ (locₛ * 𝔄))  (fst ∘ lπ))).
-      iFrame. exact.
-      rewrite (tctx_hasty_val #l2). iExists _. iSplit; [done|].
-      simpl. iFrame. iNext. iExists _. iFrame. iExists (const -[]). done.
-    - iApply proph_obs_impl; [|done]=> π.
-      move: (equal_f Eq1 π) (equal_f Eq2 π)=>/=. case (lπ π)=>/= ??->-> Imp Eq.
-      rewrite Eq in Imp. apply Imp. rewrite /alapply fmap_app. reflexivity.
-      intros. apply no_dup. done.
+    intros ?. eapply type_fn; [apply _|]=> α ??[l[l2[]]]. simpl_subst. via_tr_impl.
+    iApply ghost_read_delete; [done|]. iIntros. iApply typed_body_tctx_incl.
+    eapply ghost_update; [done|solve_typing|]. eapply tctx_incl_trans. eapply seq_fappend. unfold ghostptrtoken_ty. eapply tctx_incl_trans. eapply ghost_dummy'.
+    eapply tctx_incl_swap. iApply type_jump; [solve_typing|solve_extract|].
+    apply resolve_tctx_cons_hasty; [apply uniq_ghostptrtoken_resolve; [done|solve_typing]|apply resolve_tctx_nil].
+    move=>post [[??][?[]]]Impl[eq?]/=. rewrite eq in Impl. by apply Impl.
   Qed.
-End ghostptrtoken_insertremove.
+End ghostptrtoken_merge.
