theories/typing/lib/ghostptrtoken/ghostseq_basic.v
@@ -1,5 +1,5 @@
 From lrust.typing Require Export type.
-From lrust.typing Require Import array_util typing zst.
+From lrust.typing Require Import array_util typing logic_fn.
 From lrust.typing.lib.ghostptrtoken Require Import ghostseq.
 Set Default Proof Using "Type".
 
@@ -43,6 +43,60 @@ Section ghostseq_basic.
 
   Global Instance seq_sync {𝔄} (ty: type 𝔄) : Sync ty → Sync (ghostseq_ty ty).
   Proof. move=> ?>/=. by do 6 (f_equiv || move=>?). Qed.
+
+  Definition always_true {𝔄} (P: 𝔄 → Prop) (ty: type 𝔄) := (∀ vπ d tid vl F, (ty_own ty vπ d tid vl) -∗ (|={F}▷=>^d ⟨ π , P (vπ π) ⟩) ∗ (ty_own ty vπ d tid vl) ).
+
+  Lemma resolve_uniq_body' {𝔄} (P: 𝔄 → Prop) (ty: type 𝔄) vπ ξi d κ tid l E L q F :
+    always_true P ty → lctx_lft_alive E L κ → ↑lftN ∪ ↑prophN ⊆ F →
+    lft_ctx -∗ proph_ctx -∗ κ ⊑ ty_lft ty -∗ elctx_interp E -∗ llctx_interp L q -∗
+    uniq_body ty vπ ξi d κ tid l ={F}=∗ |={F}▷=>^(S d) |={F}=>
+      ⟨π, π (PrVar (𝔄 ↾ prval_to_inh vπ) ξi) = vπ π ∧ P (vπ π)⟩ ∗ llctx_interp L q.
+  Proof.
+    iIntros (H Alv ?) "#LFT PROPH In E L [Vo Bor] /=".
+    iMod (Alv with "E L") as (?) "[[κ κ₊] ToL]"; [solve_ndisj|].
+    iMod (bor_acc with "LFT Bor κ") as "[(%&%& ⧖ & Pc &%& ↦ & ty) ToBor]";
+      [solve_ndisj|]. iIntros "!>!>!>".
+    iDestruct (H with "ty") as "(Obs&ty)".
+    iMod (ty_own_proph with "LFT In ty κ₊") as "Upd"; [solve_ndisj|].
+    iDestruct (uniq_agree with "Vo Pc") as %[<-<-]. iCombine "Obs Upd" as "Upd".
+    iApply (step_fupdN_wand with "Upd"). iIntros "!> (Obs&>(%&%&%& ξl & Toty))".
+    iMod (uniq_resolve with "PROPH Vo Pc ξl") as "(Obs'& Pc & ξl)"; [solve_ndisj| |].
+    by eapply ty_proph_weaken. iCombine "Obs' Obs" as "$".
+    iMod ("Toty" with "ξl") as "[ty κ₊]".
+    iMod ("ToBor" with "[⧖ Pc ↦ ty]") as "[_ κ]".
+    { iNext. iExists _, _. iFrame "⧖ Pc". iExists _. iFrame. }
+    iApply "ToL". iFrame.
+  Qed.
+
+  Lemma uniq_resolve' {𝔄} (P: 𝔄 → Prop) E L κ (ty: type 𝔄) :
+    always_true P ty → lctx_lft_alive E L κ → resolve E L (&uniq{κ} ty) (λ '(a, a'), a' = a ∧ P a).
+  Proof.
+    move=>/= H??? vπ ?? vl ?. iIntros "LFT PROPH E L [In uniq]".
+    case vl as [|[[]|][]]=>//. iDestruct "uniq" as (??[Le Eq]) "uniq".
+    iMod (resolve_uniq_body' with "LFT PROPH In E L uniq") as "Upd"; [done..|].
+    iApply step_fupdN_nmono; [done|]. iApply (step_fupdN_wand with "Upd").
+    iIntros "!> >(?&$) !>". iApply proph_obs_eq; [|done]=>/= π.
+    move: (equal_f Eq π)=>/=. by case (vπ π)=>/= ??->.
+  Qed.
+
+  Lemma uniq_seq_resolve {𝔄 T} (f: 𝔄 → T) E L κ (ty: type 𝔄) :
+  (∀ vπ vπ' d d' tid tid' F, (ty_own ty vπ d tid []) -∗ (ty_own ty vπ' d' tid' []) -∗ (|={F}▷=>^d ⟨ π , f (vπ π) ≠ f (vπ' π)  ⟩) ∗ (ty_own ty vπ d tid []) ∗ (ty_own ty vπ' d' tid' []) )
+    → lctx_lft_alive E L κ → resolve E L (&uniq{κ} (ghostseq_ty ty)) (λ '(a, a'), a' = a ∧ NoDup (f <$> a)).
+  Proof.
+    intros. apply (uniq_resolve'  (λ (a: listₛ 𝔄), _)); [|done].
+    iIntros (?????) "token". iDestruct "token" as (?[->->]) "tys".
+    iAssert ((|={F}▷=>^d _) ∗ _)%I with "[tys]" as "($&?)"; [|iExists aπl; (iSplit; [|done]; done)].
+    iInduction aπl as [|aπ] "IH". iFrame "tys". iApply step_fupdN_full_intro. iApply proph_obs_true=>π/=. constructor.
+    iAssert ((|={F}▷=>^d ⟨ π , _⟩) ∗ _ ∗ _)%I with "[tys]" as "(Obs&ty&tys)"; last first.
+    iDestruct ("IH" with "tys") as "(Obs'&tys)". iCombine "Obs Obs'" as "Obs".
+    iSplitL "Obs". iApply (step_fupdN_wand with "Obs"); iIntros "(Obs&Obs')"; iCombine "Obs Obs'" as "Obs". iApply (proph_obs_impl with "Obs")=>π/=?. rewrite NoDup_cons. done. iFrame. done.
+    iClear "IH"; simpl. iInduction aπl as [|aπ'] "IH". iFrame "tys". iApply step_fupdN_full_intro. iApply proph_obs_true=>π/=. rewrite elem_of_nil. intros [].
+    iDestruct "tys" as "(ty1&ty2&tys)".
+    iDestruct (H with "ty1 ty2") as "(Obs&ty1&$)". 
+    iDestruct ("IH" with "[ty1 tys]") as "(Obs'&($&$))". iFrame. iCombine "Obs Obs'" as "Obs".
+    iApply (step_fupdN_wand with "Obs"); iIntros "(Obs&Obs')"; iCombine "Obs Obs'" as "Obs".
+    iApply (proph_obs_impl with "Obs")=>π/=?. rewrite not_elem_of_cons. done.
+  Qed.
 
   Lemma seq_resolve {𝔄} (ty: type 𝔄) Φ E L :
     resolve E L ty Φ → resolve E L (ghostseq_ty ty) (lforall Φ).
@@ -109,15 +163,15 @@ Section ghostseq_basic.
   Global Instance seq_zst {𝔄} (ty: type 𝔄) : ZST (ghostseq_ty ty).
   Proof. done. Qed.
 
-  Lemma seq_append {𝔄} (ty: type 𝔄) E L :
-  tctx_incl E L +[null_val ◁ (box (ghostseq_ty ty)); null_val ◁ (box (ghostseq_ty ty))] +[null_val ◁ (box (ghostseq_ty ty))]
+  Lemma seq_append {𝔄} (ty: type 𝔄) p1 p2 E L :
+  tctx_incl E L +[p1 ◁ (box (ghostseq_ty ty)); p2 ◁ (box (ghostseq_ty ty))] +[null_val ◁ (box (ghostseq_ty ty))]
     (λ post '-[s1; s2], post -[s1 ++ s2]).
   Proof. split. solve_proper.
     iIntros (??(s1π&s2π&[])?) "_ _ _ _ $ (ty1&ty2&true) Obs"; 
     iExists (-[λ π, _]); iFrame.
-    rewrite 3! tctx_elt_interp_zst.
-    iDestruct "ty1" as "(%&⧖&%&>(_&->)&ty1)".
-    iDestruct "ty2" as "(%&⧖'&%&>(_&->)&ty2)".
+    rewrite tctx_elt_interp_zst 2! tctx_elt_interp_zst''.
+    iDestruct "ty1" as (???) "(⧖&%&>(_&->)&ty1)".
+    iDestruct "ty2" as (???) "(⧖'&%&>(_&->)&ty2)".
     iCombine "⧖ ⧖'" as "⧖". simpl.
     iModIntro. iExists _. iFrame. iNext. iExists _.
     iSplit. iPureIntro. split; [done|]. fun_ext. intros. rewrite -fmap_app. done.
@@ -126,38 +180,67 @@ Section ghostseq_basic.
     (iApply ty_own_depth_mono; [|done]); lia.
   Qed.
 
-  Lemma seq_new {𝔄} (ty: type 𝔄) E L :
-  tctx_incl E L +[null_val ◁ (box ())] +[null_val ◁ (box (ghostseq_ty ty))]
+  Lemma seq_fappend {𝔄} (ty: type 𝔄) p1 p2 E L :
+  tctx_incl E L +[p1 ◁ (box (ghostseq_ty ty)); p2 ◁ (box (ghostseq_ty ty))] +[null_val ◁ (box (ghostseq_ty ty))]
+    (λ post '-[s1; s2], post -[s2 ++ s1]).
+  Proof.
+    eapply tctx_incl_ext. eapply tctx_incl_trans. apply tctx_incl_swap. apply seq_append. done.
+  Qed.
+
+  Lemma seq_new {𝔄} (ty: type 𝔄) p E L :
+  tctx_incl E L +[p ◁ (box ())] +[null_val ◁ (box (ghostseq_ty ty))]
     (λ post '-[_], post -[[]]).
   Proof. split. solve_proper.
     iIntros (??(?&[])?) "_ _ _ _ $ (⧖&true) Obs"; 
     iExists (-[λ π, _]); iFrame.
-    rewrite tctx_elt_interp_zst tctx_hasty_val.
-    iDestruct "⧖" as ([|?]) "(⧖&?)"; [done|].
+    rewrite tctx_elt_interp_zst'' tctx_elt_interp_zst.
+    iDestruct "⧖" as (???) "(⧖&_)".
     iModIntro. iExists _. iFrame. iNext. iExists []. iSplit; done.
   Qed.
 
-  (* Lemma seq_split {𝔄 𝔄l} (ty: type 𝔄) `{!Copy ty} (T: tctx 𝔄l) E L :
-  tctx_incl E L (null_val ◁ (box (ghostseq_ty ty)) +:: T) (null_val ◁ (box (ghostseq_ty ty)) +:: null_val ◁ (box (ghostseq_ty ty)) +:: T)
-    (λ post '(s -:: al), ∃ s1 s2, s1 ++ s2 = s ∧ post (s1 -:: s2 -:: al)).
+  Lemma seq_split {𝔄} (ty: type 𝔄) p1 p2 E L :
+  tctx_incl E L +[p1 ◁ (box (ghostseq_ty ty)); p2 ◁ (box (ghost int))] +[null_val ◁ (box (ghostseq_ty ty)); null_val ◁ (box (ghostseq_ty ty))]
+    (λ post '-[s; i], exists (n: nat), (Z.of_nat n) = i ∧ post -[(take n s); (drop n s)]).
   Proof. split. solve_proper.
-    iIntros (??(sπ&lπ)?) "_ PROPH _ _ $ (ty&?) Obs".
-    rewrite tctx_elt_interp_zst.
-    iDestruct "ty" as "(%&⧖&%&>(_&->)&ty1)".
-    iMod (proph_obs_sat with "PROPH Obs") as "(%&%&%&%&%)"; [done|].
-    iExists ((λ π, _) -:: lπ); iFrame. *)
-    
-    
-    (* iDestruct "ty2" as "(%&⧖'&%&>(_&->)&ty2)".
-    iCombine "⧖ ⧖'" as "⧖". simpl.
-    iModIntro. iExists _. iFrame. iNext. iExists _.
-    iSplit. iPureIntro. split; [done|]. fun_ext. intros. rewrite -fmap_app. done.
-    rewrite big_sepL_app. iSplitL "ty1"; 
-    (iApply (big_sepL_impl with "[-]"); [done|]); iIntros "!> **";
-    (iApply ty_own_depth_mono; [|done]); lia.
-  Qed. *)
+    iIntros (??(sπ&zπ&[])?) "_ PROPH _ _ $ (ty&tyz&?) #Obs".
+    rewrite 2! tctx_elt_interp_zst''.
+    iDestruct "ty" as (???) "(#⧖&%&>(_&->)&ty)".
+    iDestruct "tyz" as (???) "(_&>(_&%&%&->))". simpl.
+    iMod (proph_obs_sat with "PROPH Obs") as "(%&%&<-&%)"; [done|].
+    set aπl1 := (take n aπl). set aπl2 := (drop n aπl).
+    replace aπl with (aπl1 ++ aπl2); last first. apply take_drop.
+    iDestruct "ty" as "(ty1&ty2)". iModIntro.
+    iExists -[(lapply aπl1); (lapply aπl2)]. simpl. iFrame. rewrite 2! tctx_elt_interp_zst.
+    iSplit. iSplitL "ty1"; iExists _; iFrame "⧖"; iExists _; iFrame; done.
+    iApply (proph_obs_impl with "Obs")=>π/=. intros (?&->%inj&?).
+    rewrite /lapply -fmap_take -fmap_drop take_drop in H2. done. intros ??. apply Nat2Z.inj.
+  Qed.
 
-  Lemma seq_one `{!Inhabited 𝔄} (ty: type 𝔄) `{!ZST ty} E L : eqtype E L (!{λ (l: listₛ 𝔄), length l = 1} (ghostseq_ty ty)) ty (λ (l: list 𝔄), l !!! 0) (λ x, [x]).
+  Lemma seq_singleton {𝔄} (ty: type 𝔄) `{!ZST ty} p E L :
+  tctx_incl E L +[p ◁ (box ty)] +[null_val ◁ (box (ghostseq_ty ty))]
+    (λ post '-[x], post -[[x]]).
+  Proof. split. solve_proper.
+    iIntros (??(?&[])?) "_ _ _ _ $ (ty&true) Obs"; 
+    iExists (-[λ π, _]); iFrame.
+    rewrite tctx_elt_interp_zst'' tctx_elt_interp_zst.
+    iDestruct "ty" as (???) "(⧖&ty)".
+    iModIntro. iExists _. iFrame. iNext. iExists [_]. iSplit; [done|]. iFrame. done.
+  Qed.
+
+  Lemma seq_destruct_singleton {𝔄} (ty: type 𝔄) `{!ZST ty} p E L :
+  tctx_incl E L +[p ◁ (box (ghostseq_ty ty))] +[null_val ◁ (box ty)]
+    (λ post '-[s], exists (x: 𝔄), s = [x] ∧ post -[x]).
+  Proof. split. solve_proper.
+    iIntros (??(sπ&[])?) "_ PROPH _ _ $ (ty&true) #Obs".
+    iMod (proph_obs_sat with "PROPH Obs") as %(?&?&sat&_); [done|]. unfold phd in sat. simpl in sat.
+    iExists (-[λ π, match (sπ π) with | [x] => x | _ => x0 end]); iFrame.
+    rewrite tctx_elt_interp_zst'' tctx_elt_interp_zst.
+    iDestruct "ty" as (???) "(⧖&ty)". iModIntro. iSplitL.
+    iExists _. iFrame. iNext. iDestruct "ty" as ([|?[|]][_->]) "ty"; try done. iDestruct "ty" as "($&_)".
+    iApply (proph_obs_impl with "Obs")=>π/=[?[->?]]. done.
+  Qed.
+
+  (* Lemma seq_one `{!Inhabited 𝔄} (ty: type 𝔄) `{!ZST ty} E L : eqtype E L (!{λ (l: listₛ 𝔄), length l = 1} (ghostseq_ty ty)) ty (λ (l: list 𝔄), l !!! 0) (λ x, [x]).
   Proof. 
     split; iIntros; iModIntro; iIntros "_".
     - iSplit. iPureIntro. split. rewrite zero_size. done.
@@ -172,32 +255,53 @@ Section ghostseq_basic.
       iSplit. iApply lft_incl_refl.
       iSplit; iModIntro; iIntros; (iSplit; [by iApply proph_obs_s_true|]); iExists [vπ];
       [iDestruct (zst_size_eq with "[$]") as %->|]; simpl; (iSplit; [done|]); iSplit; done.
+  Qed. *)
+
+  Lemma seq_cons {𝔄} (ty: type 𝔄) `{!ZST ty} p1 p2 E L :
+  tctx_incl E L +[p1 ◁ (box (ghostseq_ty ty)); p2 ◁ (box ty)] +[null_val ◁ (box (ghostseq_ty ty))]
+    (λ post '-[s; v], post -[v :: s]).
+  Proof.
+    eapply tctx_incl_ext. eapply tctx_incl_trans. eapply tctx_incl_tail. apply seq_singleton. done. 
+    eapply seq_fappend. move=>?[?[?[]]]/=. done.
   Qed.
 
-  (* Lemma seq_perm {𝔄}  g ty E L :
+  Lemma seq_remove {𝔄} (ty: type 𝔄) `{!ZST ty} p1 p2 E L :
+  tctx_incl E L +[p1 ◁ (box (ghostseq_ty ty)); p2 ◁ (box (ghost int))] +[null_val ◁ (box (ghostseq_ty ty)); null_val ◁ (box (ty))]
+    (λ post '-[s; i], exists (n: nat) (v: 𝔄), (Z.of_nat n) = i ∧ s !! n = Some v ∧ post -[base.delete n s; v]).
+  Proof.
+    eapply tctx_incl_ext. eapply tctx_incl_trans. eapply tctx_incl_tail. eapply copy_ghost. done. apply ghost_copy.
+    eapply tctx_incl_trans. eapply (tctx_incl_app +[_; _] _ +[_] _). apply seq_split.
+    eapply (logic_fn_ghost_tctx_incl' (𝔄l:=[]) -[p2] _ +[]). eapply (plain_logic_fn +[_] _ (λ '-[x], (1: Zₛ))).
+    eapply tctx_incl_trans. eapply tctx_incl_tail. eapply tctx_incl_trans. apply seq_split.
+    eapply tctx_incl_trans. apply tctx_incl_swap. eapply tctx_incl_tail. apply seq_destruct_singleton. done.
+    eapply (tctx_incl_frame_r +[_; _] +[_]). eapply seq_append.
+    move=>?[s[?[]]]/=. rewrite /trans_app /trans_tail /trans_upper. simpl.
+    f_equiv. f_equiv. setoid_rewrite delete_take_drop. setoid_rewrite drop_drop. setoid_rewrite Nat.add_comm. split.
+    move=>[x[<-[lookup ?]]]. split. done. exists 1%nat. split. lia. exists x. simpl.
+    split. rewrite -(take_drop_middle _ _ _ lookup) drop_app_alt. done. rewrite take_length. remember (lookup_lt_Some _ _ _ lookup). 
+    rewrite min_l. done. apply (le_trans _ (S a) _). lia. done. done.
+    intros [<-[? [->%Nat2Z.inj [x[td ?]]]]]. exists x. split. done. simpl in td.
+    split. remember (lookup_drop s a 0) as eq. clear Heqeq.
+    rewrite Nat.add_comm in eq. rewrite -eq. remember (drop a s) as d; destruct d. done. injection td=><-. done. done. 
+  Qed.
+
+      (* Lemma seq_perm {𝔄}  g ty E L :
    (∀ x, f x ≡ₚ x) → subtype E L (ghostseq_ty ty) (ghostseq_ty ty) f.
   Proof. move=> [??]. split; by apply seq_subtype. Qed. *)
-
+  
   (* Rust's GhostSeq::new *)
   Definition ghostseq_new: val :=
     fn: [] :=
-      let: "r" := new [ #0] in
-      return: ["r"].
+      Skip;;
+      return: [ #null_loc].
 
   Lemma ghostseq_new_type {𝔄} (ty: type 𝔄) :
-    typed_val ghostseq_new (fn(∅) → ghostseq_ty ty) (λ post _, post []).
+    typed_val ghostseq_new (fn(∅) → ghostseq_ty ty) (λ (post: (list 𝔄) → _) '-[], post []).
   Proof.
-    eapply type_fn; [apply _|]=> _ ???. simpl_subst.
-    iIntros (???) "_ #TIME _ _ _ Na L C _ Obs". iMod persistent_time_receipt_0 as "⧖".
-    wp_bind (new _). iApply (wp_persistent_time_receipt with "TIME ⧖"); [done|].
-    iApply wp_new; [done..|]. iIntros "!>" (l) "[† _] ⧖". wp_seq.
-    do 2 wp_seq.
-    rewrite cctx_interp_singleton.
-    iApply ("C" $! [# #_] -[const []] with "Na L [-Obs] Obs"). iSplit; [|done].
-    iExists _, _. do 2 (iSplit; [done|]). rewrite/= freeable_sz_full split_mt_seq. 
-    iFrame "†". iNext. iExists []. iSplit.
-    iPureIntro. done.
-    rewrite heap_mapsto_vec_nil. iSplit; done.
+    eapply type_fn; [apply _|]=> _ ???. simpl_subst. via_tr_impl.
+    iApply ghost_dummy. iApply typed_body_tctx_incl. eapply seq_new.
+    iApply type_jump; [solve_typing|solve_extract|solve_typing].
+    move=>π//=.
   Qed.
 End ghostseq_basic.
 
