theories/typing/lib/ghostptrtoken/ghostptrtoken_insertremove.v
@@ -1,6 +1,6 @@
 From lrust.typing Require Export type.
-From lrust.typing Require Import uniq_util typing ptr.
-From lrust.typing.lib Require Import ghostptrtoken.ghostptrtoken ghostptrtoken.heap_util.
+From lrust.typing Require Import uniq_util typing ptr ghost.
+From lrust.typing.lib.ghostptrtoken Require Import ghostptrtoken_basic ghostseq_basic permdata_basic.
 Set Default Proof Using "Type".
 
 Open Scope nat.
@@ -11,64 +11,23 @@ Section ghostptrtoken_insertremove.
 
   Definition ghostptrtoken_insert {𝔄} (ty: type 𝔄) : val :=
     fn: ["t"; "b"] :=
+      Skip;;
       delete [ #1; "t"];;
       return: ["b"].
 
-  (* Rust's GhostPtrToken::insert *)
   Lemma ghostptrtoken_insert_type {𝔄} (ty: type 𝔄) :
    (ty.(ty_size) > 0) → typed_val (ghostptrtoken_insert ty) (fn<α>(∅; &uniq{α} (ghostptrtoken_ty ty), box ty) → ptr)
       (λ post '-[(al, al'); a], forall ptr, (list_to_gmap al') = <[ptr:=a]>(list_to_gmap al) → (list_to_gmap al) !! ptr = None → post ptr).
-  Proof. intros.
-    eapply type_fn; [apply _|]=> α ??[l[x[]]]. simpl_subst.
-    iIntros (?(lπ & bπ &[]) ?) "#LFT #TIME #PROPH #UNIQ #E Na L C /=(l & x &_) #Obs".
-    rewrite !tctx_hasty_val. iDestruct "l" as ([|dl]) "[_ l]"=>//.
-    case l as [[|l|]|]=>//. iDestruct "l" as "[(%ll & >↦l & [#LftIn uniq]) †l]".
-    case ll as [|[[|l'|]|][]]; try by iDestruct "uniq" as ">[]".
-    iDestruct "x" as ([|dx]) "[⧖x x]"=>//. case x as [[|x|]|]=>//=.
-    iDestruct "x" as "[x' †x]".
-     wp_bind (delete _). rewrite freeable_sz_full.
-    iApply ((wp_delete [ #l'])with "[↦l †l]"); [done| by iFrame|]. 
-    iNext. iIntros.
-    iDestruct "x'" as (?) "(↦x&x')".
-    case dx as [|dx]=>//=. case vl as [|[[|p|]|][]]=>//=.
-    iDestruct "x'" as "(x'&†x')".
-    iDestruct "uniq" as (du ξi [? Eq2]) "[Vo Bor]".
-    move: Eq2. set ξ := PrVar _ ξi=> Eq2.
-    iMod (lctx_lft_alive_tok α with "E L") as (?) "(α & L & ToL)"; [solve_typing..|].
-    iMod (bor_acc with "LFT Bor α") as "[(%&%& ⧖u & Pc & ↦token) ToBor]"; [done|].
-    wp_seq. iDestruct (uniq_agree with "Vo Pc") as %[<-<-].
-    rewrite split_mt_token.
-    iDestruct "↦token" as (aπl Eq1) "(↦l & ↦tys & †)".
-    iCombine "⧖u ⧖x" as "#⧖". simpl.
-    iMod (uniq_update with "UNIQ Vo Pc") as "[Vo Pc]"; [done|].
-    iDestruct ((plain_entails_r (ghost_ptr_token_no_dup' _ ((p, bπ)::aπl) (du `max` (S dx)) _ H)) with "[↦tys x']") as "(↦tys&>%no_dup)".
-    { replace (du `max` (S dx)) with (S ((pred du) `max` dx)); [|lia]. simpl. 
-    iSplitL "x'". iNext. iApply (ty_own_mt_depth_mono with "x'"); lia.
-    iApply (big_sepL_impl with "↦tys"). iModIntro. iIntros (?[??]?) "H". destruct du; [done|].
-    iApply (ty_own_mt_depth_mono with "H"); lia. }
-    iAssert ((l' ↦∗: (ghostptrtoken_ty ty).(ty_own) _ _ tid))%I with "[↦l ↦tys † †x']" as "own".
-    iApply split_mt_token. iExists ((p, bπ)::aπl). 
-    rewrite freeable_sz_full. iFrame. done.
-    iMod ("ToBor" with "[own Pc]") as "[Bor α]".
-    iDestruct (bi.later_intro with "own") as "own". 
-    iNext. iExists _, _. setoid_rewrite split_mt_token. iFrame "⧖ Pc".
-    iClear "#". iStopProof. do 11 f_equiv.
-    iMod ("ToL" with "α L") as "L".
-    set lπ' := λ π, ((alapply ((p, bπ)::aπl) π), π ξ).
-    iApply (type_type +[#l' ◁ &uniq{α} (ghostptrtoken_ty ty); #x ◁ box ptr] -[lπ'; const p]
-    with "[] LFT TIME PROPH UNIQ E Na L C [-] []").
-    - iApply type_jump; [solve_typing|solve_extract|solve_typing].
-    - iSplitL "Vo Bor"; [|iSplitL; [|done]]. rewrite (tctx_hasty_val #l').
-      iExists _. iSplit; [done|]. 
-      iSplit; [done|]. fold max. iExists _, _. rewrite /uniq_body.
-      rewrite (proof_irrel (@prval_to_inh (listₛ (locₛ * 𝔄)) (fst ∘ lπ')) (@prval_to_inh (listₛ (locₛ * 𝔄))  (fst ∘ lπ))).
-      iFrame. exact.
-      rewrite (tctx_hasty_val #x). iExists _. iSplit; [done|].
-      simpl. iFrame. iNext. iExists _. iFrame. iExists p. done.
-    - iApply proph_obs_impl; [|done]=> π.
-      move: (equal_f Eq1 π) (equal_f Eq2 π)=>/=. case (lπ π)=>/= ??->-> Imp Eq.
-      apply Imp. rewrite Eq. reflexivity.
-      apply not_elem_of_list_to_map_1. rewrite -list_fmap_compose.  inversion_clear no_dup. done.
+  Proof.
+    intros ?. eapply type_fn; [apply _|]=> α ??[l[l2[]]]. simpl_subst. via_tr_impl.
+    iApply ghost_read_delete; [done|]. iIntros. iApply typed_body_tctx_incl.
+    eapply ghost_update; [done|solve_typing|]. 
+    eapply tctx_incl_trans. eapply (tctx_incl_frame_l _ _ +[_]). eapply tctx_incl_trans. eapply permdata_from_box. eapply tctx_incl_swap.
+    simpl. eapply (tctx_incl_frame_r +[_; _] +[_] +[_]). eapply seq_cons. done.
+    iApply type_jump; [solve_typing|solve_extract|].
+    apply resolve_tctx_cons_hasty; [apply uniq_ghostptrtoken_resolve; [lia|solve_typing]|apply resolve_tctx_nil].
+    move=>post [[tc tf][v []]]Impl l' [eq nodup]/=. rewrite eq in Impl. apply Impl. done.
+    apply not_elem_of_list_to_map_1. inversion_clear nodup. done.
   Qed.
 
   Definition ghostptrtoken_remove {𝔄} (ty: type 𝔄) : val :=
